

1. CB4.32

a. $Y|A \sim \text{POISS}(A)$ $A \sim \text{Gamma}(\alpha, \beta)$ Find Y , $E(Y)$, $\text{Var}(Y)$, and $Y \sim \text{NEGBINOM}(\alpha = 1, 2, 3, \dots)$

$$f_Y = \int_0^\infty f_Y(y|a) f_A(a) da = \int_0^\infty \frac{a^y e^{-a}}{y!} \cdot \frac{1}{\Gamma(\alpha)\beta^\alpha} a^{\alpha-1} e^{-a/\beta} da = \frac{1}{y! \Gamma(\alpha) \beta^\alpha} \int_0^\infty \underbrace{a^{(\alpha+y)-1} e^{-a(1+1/\beta)}}_{\text{KERNEL OF GAMMA: } \alpha = \alpha+y, \beta = \frac{1}{1+1/\beta}} da$$

$$f_Y = \frac{\Gamma(\alpha+y) \left(\frac{1}{1+1/\beta}\right)^{\alpha+y}}{y! \Gamma(\alpha) \beta^\alpha}$$

$$E_Y = E_A(E_{Y|A}(Y|A)) = E_A(A) = \alpha\beta \quad \underline{E_Y = \alpha\beta}$$

$$\text{Var}_Y = E(\text{Var}(Y|A)) + \text{Var}(E(Y|A)) = E(A) + \text{Var}(A) = \alpha\beta + \alpha\beta^2 = \text{Var}_Y$$

$$\text{If } \alpha \text{ is INTEGER, } f_Y = \frac{(\alpha+y)!}{y! \alpha!} \left(\frac{\beta}{1+\beta}\right)^{\alpha+y} \cdot \frac{1}{\beta} = \binom{y+\alpha-1}{y} \cdot \left(\frac{\beta}{1+\beta}\right)^y \left(\frac{1}{1+\beta}\right)^\alpha = \underline{\text{NEGBINOM}(\alpha, \frac{1}{1+\beta})}$$

b. $Y|N \sim \text{BINOM}(N, p)$ $N|A \sim \text{POISS}(A)$ $A \sim \text{Gamma}(\alpha, \beta)$

$$f_{Y|N} = P(Y=y|A) = P(Y=y|N=n, \lambda) P(N=n|A) = \sum_{n=y}^{\infty} \binom{n}{y} p^y (1-p)^{n-y} \frac{e^{-\lambda} \lambda^n}{n!}$$

$$= \sum_{n=y}^{\infty} \frac{1}{y!(n-y)!} \left(\frac{p}{1-p}\right)^y ((1-p)\lambda)^{n-y} e^{-\lambda} = \frac{e^{-\lambda}}{y!} \left(\frac{p}{1-p}\right)^y \sum_{m=0}^{\infty} \frac{((1-p)\lambda)^{m+y}}{m!} = \frac{e^{-\lambda}}{y!} \left(\frac{p(1-p)\lambda}{1-p}\right)^y \sum_{m=0}^{\infty} \frac{((1-p)\lambda)^m}{m!}$$

$$= \frac{e^{-\lambda}}{y!} (p\lambda)^y e^{(1-p)\lambda} = \frac{(p\lambda)^y e^{-p\lambda}}{y!} = \text{POISS}(p\lambda)$$

$\therefore f_{Y|N} \sim \text{POISS}$ WHICH IS THE SAME START AS (a), BUT WITH $p\lambda$ INSTEAD OF β :

$$f_Y = \frac{(\alpha+y)!}{y! \Gamma(\alpha) (\beta p)^{\alpha+y}} \left(\frac{p\lambda}{1+p\lambda}\right)^{\alpha+y}$$

2. 4.35 $X|P \sim \text{BINOM}(n, p)$ $P \sim \text{BETA}(\alpha, \beta)$

$$a. \text{Var}(X) = E(\text{Var}(X|P)) + \text{Var}(E(X|P)) = E(nP(1-P)) + \text{Var}(nP) = n E(P(1-P)) + n(n-1) \text{Var}(P)$$

$$= n E(p) (1-E(p)) + n(n-1) \text{Var}(p) = \underline{\text{Var}(X)}$$

b. $Y|A \sim \text{POISSON}(A)$ $A \sim \text{Gamma}(\alpha, \beta)$

$$\text{As shown in 4.32 (a), } \text{Var}(Y) = \alpha\beta + \alpha\beta^2 \quad E(A) = \alpha\beta \Rightarrow \underline{\text{Var}(Y) = E(A) + \frac{1}{\alpha} E(A)^2} = \mu + \frac{1}{\alpha} \mu^2 \quad \text{WHERE } \mu = E(A)$$

3. X, Y HAVE FINITE VARIANCES. PROVE:

$$\begin{aligned} a) E(XY) &= E(X E(Y|X)) & E(XY) &= \iint xy f_{xy} dx dy = \iint xy f_{y|x} f_x dx dy \\ & & &= \int x f_x \left[\int y f_{y|x} dy \right] dx = \int x f_x E(Y|X) dx = E[X E(Y|X)] \end{aligned}$$

$$b) \text{Cov}(X, Y) = \text{Cov}(X, E(Y|X))$$

$$\text{Cov}(X, Y) = \underline{E(XY) - E(X)E(Y)}$$

$$\text{Cov}(X, E(Y|X)) = E(X E(Y|X)) - E(X) E(E(Y|X)) = E(XY) - \underline{E(X)E(Y)}$$

c) $X, Y - E(Y|X)$ ARE UNCORRELATED: $Cov(X, Y - E(Y|X)) = E(XY - XE(Y|X)) - E(X)E(Y - E(Y|X))$
 $= E(XY) - E(X)E(Y) - E(X)E(Y) + E(X)E(E(Y|X)) = 0 - E(X)E(Y) + E(X)E(Y) = 0$

4. $F_{END} E(x)$

$$a) X|Y \sim \text{BINOM}(n, Y) \quad Y \sim \text{BETA}(a, b) \quad E(X) = E_Y(E_{X|Y}(X|Y)) = E_Y(nY) = nE_Y(Y) = \frac{na}{a+b}$$

b) $X|Y \sim \text{Exp}(Y)$ $Y \sim \text{Gamma}(a, b)$ $E(X) = E_Y(E_{X|Y}(X|Y)) = E_Y(Y) = \underline{a/b}$

5. Find $VAR(x)$ for $y(x)$

$$\begin{aligned} \text{Var}(x) &= E(\text{Var}(x|Y)) + \text{Var}(E(x|Y)) = E(nY(1-Y)) + \text{Var}(nY) = n E(Y - Y^2) + n(n-1) \text{Var}(Y) \\ &= \frac{n a}{a+b} + \frac{n(n-1) a b}{(a+b)^2 (a+b+1)} - n E(Y^2) \\ &\quad \text{L.S.} = \text{Var}(Y) + E(Y)^2 = \frac{a(a+1)}{(a+b)(a+b+1)} \\ &= \frac{n a}{a+b} \left[1 + \frac{(n-1)b}{(a+b)(a+b+1)} - \frac{a+1}{a+b+1} \right] \end{aligned}$$

6. $P(Y=1)=.3$ $P(Y=2)=.7$ $X|Y = \text{POISSON}(Y)$ Find $M_X(t)$

$$X \sim .3 \text{ Poiss}(1) + .7 \text{ Poiss}(2) \quad M_X(t) = M_{\text{Poiss}(1)}(.3t) \cdot M_{\text{Poiss}(2)}(.7t) = e^{(e^{.3t} - 1)} \cdot e^{2(e^{.7t} - 1)}$$

$$= e^{e^{.3t} + 2e^{.7t} - 3} = M_X(t)$$

7, CB 4.41 Show any r.v. is uncorrelated with a constant

NEED TO SHOW: $\text{Cov}(X, c) = 0$ $\text{Cov}(X, c) = E(Xc) - E(X)E(c) = cE(X) - cE(X) = 0 = \text{Cov}(X, c)$
 $\therefore \text{CORR} = \frac{\text{Cov}}{\sigma\sigma} = 0$

8. CB 4.42 $X \perp Y$, $\mu_X, \mu_Y, \sigma_X^2, \sigma_Y^2$ Express $\text{Corr}(XY, Y)$ in those terms

$$\text{Corr}(X, Y) = \frac{\text{Cov}(X, Y)}{\sigma_X \sigma_Y} \quad \text{Cov}(X, Y) = E(XY) - E(X)E(Y)$$

x, y

$$\text{Var}(XY) = E(X^2 Y^2) - E(XY)^2 = E(X^2) E(Y^2) - E(X)^2 E(Y)^2 = (\text{Var}(X) + \mu_X^2) (\text{Var}(Y) + \mu_Y^2) - \mu_X^2 \mu_Y^2$$

$$E(X^2) = \text{Var}(X) + E(X)^2$$

$$\text{Var}(XY) = \sigma_X^2 \sigma_Y^2 + \sigma_X^2 \mu_Y + \sigma_Y^2 \mu_X + \mu_X^2 \mu_Y^2 - \mu_X^2 \mu_Y^2 = \sigma_X^2 \sigma_Y^2 + \sigma_X^2 \mu_Y + \sigma_Y^2 \mu_X$$

$$E(XY) = E(X)E(Y) = \mu_X \mu_Y \quad E(Y) = \mu_Y$$

$$E(XY^2) = E(X) E(Y^2) = E(X) (\text{Var}(Y) + E(Y)^2) = \mu_X (\sigma_Y^2 + \mu_Y^2)$$

$$\text{Cov}(XY, Y) = \mu_X \sigma_Y^2 + \mu_X \mu_Y^2 - \mu_X \mu_Y^2 = \mu_X \sigma_Y^2$$

$$\text{Corr}(XY, Y) = \frac{\mu_X \sigma_Y^2}{\sigma_Y (\sigma_X^2 \sigma_Y^2 + \sigma_X^2 \mu_Y + \sigma_Y^2 \mu_X)^{1/2}} = \frac{\mu_X \sigma_Y}{(\sigma_X^2 \sigma_Y^2 + \sigma_X^2 \mu_Y + \sigma_Y^2 \mu_X)^{1/2}}$$

9. CB 4.43 X_1, X_2, X_3 UNCORRELATED, μ, σ^2 FIND $\text{Cov}(X_1 + X_2, X_2 + X_3)$; $\text{Cov}(X_1 + X_2, X_1 - X_2)$

$$\begin{aligned} \text{a. } \text{Cov}(X_1 + X_2, X_2 + X_3) &= E[(X_1 + X_2)(X_2 + X_3)] - E(X_1 + X_2)E(X_2 + X_3) = E[X_1 X_2 + X_1 X_3 + X_2^2 + X_2 X_3] - (E(X_1) + E(X_2))(E(X_2) + E(X_3)) \\ &= E(X_1 X_2) + E(X_1 X_3) + E(X_2^2) + E(X_2 X_3) - (\mu + \mu)(\mu + \mu) = E(X_1)E(X_2) + E(X_1)E(X_3) + \text{Var}(X_2) + E(X_2)E(X_3) - 4\mu^2 \\ &= \mu^2 + \mu^2 + \sigma^2 + \mu^2 + \mu^2 - 4\mu^2 = \sigma^2 \end{aligned}$$

$$\text{Cov}(X_1 + X_2, X_2 + X_3) = \sigma^2$$

$$\begin{aligned} \text{b. } \text{Cov}(X_1 + X_2, X_1 - X_2) &= E(X_1^2 - X_1 X_2 + X_1 X_2 - X_2^2) - (E(X_1) + E(X_2))(E(X_1) - E(X_2)) = E(X_1^2) - E(X_2^2) - (\mu + \mu)(\mu - \mu) \\ &= \text{Var}(X_1) + E(X_1)^2 - \text{Var}(X_2) - E(X_2)^2 - (2\mu)(0) = \sigma^2 + \mu^2 - \sigma^2 - \mu^2 - 0 = 0 \end{aligned}$$

$$\text{Cov}(X_1 + X_2, X_1 - X_2) = 0$$

10. CB 4.65 PROVE COV. INEQUALITY BY GENERALIZING: $E(g(X)(X - \mu)) \geq 0$

PROVE: LET $X \perp Y$ $g = (g(X) - g(Y))(h(X) - h(Y))$

$$\text{a) FOR } g(X) \text{ MONO} + ; h(X) \text{ MONO} - : E(g(X)h(X)) \leq E(g(X))E(h(X))$$

$$E(g) = E[(g(X) - g(Y))(h(X) - h(Y))] = [E(g(X)) - E(g(Y))][E(h(X)) - E(h(Y))]$$

WHEN $Y = X$: $E(g) = 0$

$$Y > X: E(g(Y)) \geq E(g(X)), E(h(Y)) \leq E(h(X)): E(g) = [\text{NEGATIVE}][\text{POSITIVE}] \therefore E(g) \leq 0$$

$$Y < X: E(g(Y)) \leq E(g(X)), E(h(Y)) \geq E(h(X)): E(g) = [\text{POSITIVE}][\text{NEGATIVE}] \therefore E(g) \leq 0$$

$$E(g) \leq 0 \therefore E[(g(X) - g(Y))(h(X) - h(Y))] \leq 0 \quad E[g(X)h(X) - g(X)h(Y) - g(Y)h(X) + g(Y)h(Y)] \leq 0$$

$$-E[g(X)h(Y)] - E[g(Y)h(X)] + E[g(Y)h(Y)] \leq 0$$

$$E[g(x)h(x)] = E[g(x)h(y)] + E[g(y)h(x)] - E[g(y)h(y)] = E(g(x))E(h(x))$$

$$\therefore \underline{E[g(x)h(x)] \leq E[g(x)] E[h(x)]}$$

b) For $g(x), h(x)$ BOTH MONO + or - : $E(g(x)h(x)) \geq E(g(x))E(h(x))$

WHEN $y=x$: $E(q) \geq 0$

MONOT: $y > x$: $E(g(y)) \geq E(g(x)), E(h(y)) \geq E(h(x))$: $E(q) = [\text{NEGATIVE}][\text{NEGATIVE}] \therefore E(q) \geq 0$

$y < x$: $E(g(y)) \leq E(g(x)), E(h(y)) \leq E(h(x))$: $E(q) = [\text{POSITIVE}][\text{POSITIVE}] \therefore E(q) \geq 0$

MONOT: $y < x$: $E(g(y)) \geq E(g(x)), E(h(y)) \geq E(h(x))$: $E(q) = [\text{NEGATIVE}][\text{NEGATIVE}] \therefore E(q) \geq 0$

$y > x$: $E(g(y)) \leq E(g(x)), E(h(y)) \leq E(h(x))$: $E(q) = [\text{POSITIVE}][\text{POSITIVE}] \therefore E(q) \geq 0$

WE CAN DO THE SAME EXPECTATION MOVEMENT FROM (a) TO SHOW

$$\underline{E[g(x)h(x)] \geq E[g(x)]E[h(x)]}$$